LambdaP.lean
@@ -9,3 +9,4 @@ import LambdaP.Lemmas.Subst
 import LambdaP.Soundness.Store
 import LambdaP.Soundness.Den
 import LambdaP.Soundness.PathLemmas
+import LambdaP.Soundness.DenLemmas
